Fiddling with proofs of equivalence, but sequence literals and `seq_of_list` are proving annoying

vale/code/crypto/sha/SHA_helpers.fst
@@ -56,8 +56,59 @@ let make_hash_properties (abef cdgh:quad32) :
   assert_norm(hash'.[6] == uint_to_t cdgh.lo1); 
   assert_norm(hash'.[7] == uint_to_t cdgh.lo0);
   ()
-         
-  
+
+let shuffle_core_properties (a:hash_alg) (block:block_w a) (hash:hash_w a) (t:counter{t < size_k_w a}) :
+    Lemma(let h = shuffle_core a block hash t in
+          let a0 = hash.[0] in
+          let b0 = hash.[1] in
+          let c0 = hash.[2] in
+          let d0 = hash.[3] in
+          let e0 = hash.[4] in
+          let f0 = hash.[5] in
+          let g0 = hash.[6] in
+          let h0 = hash.[7] in
+          let t1 = word_add_mod a h0 (word_add_mod a (_Sigma1 a e0) (word_add_mod a (_Ch a e0 f0 g0) (word_add_mod a (k0 a).[t] (ws a block t)))) in
+          let t2 = word_add_mod a (_Sigma0 a a0) (_Maj a a0 b0 c0) in         
+          h.[0] == word_add_mod a t1 t2 /\
+          h.[1] == a0 /\
+          h.[2] == b0 /\
+          h.[3] == c0 /\
+          h.[4] == word_add_mod a d0 t1 /\
+          h.[5] == e0 /\
+          h.[6] == f0 /\
+          h.[7] == g0)
+  =
+  let h = shuffle_core a block hash t in
+  let a0 = hash.[0] in
+  let b0 = hash.[1] in
+  let c0 = hash.[2] in
+  let d0 = hash.[3] in
+  let e0 = hash.[4] in
+  let f0 = hash.[5] in
+  let g0 = hash.[6] in
+  let h0 = hash.[7] in
+  let t1 = word_add_mod a h0 (word_add_mod a (_Sigma1 a e0) (word_add_mod a (_Ch a e0 f0 g0) (word_add_mod a (k0 a).[t] (ws a block t)))) in
+  let t2 = word_add_mod a (_Sigma0 a a0) (_Maj a a0 b0 c0) in         
+  assert(h.[0] == word_add_mod a t1 t2);
+  assert(h.[1] == a0);
+  assert(h.[2] == b0);
+  assert(h.[3] == c0);
+  assert(h.[4] == word_add_mod a d0 t1);
+  assert(h.[5] == e0);
+  assert(h.[6] == f0);
+  assert(h.[7] == g0);
+//  assert_norm(h.[0] == word_add_mod a t1 t2);
+//  assert_norm(h.[1] == a0);
+//  assert_norm(h.[2] == b0);
+//  assert_norm(h.[3] == c0);
+//  assert_norm(h.[4] == word_add_mod a d0 t1);
+//  assert_norm(h.[5] == e0);
+//  assert_norm(h.[6] == f0);
+//  assert_norm(h.[7] == g0);
+  ()
+
+
+//#push-options "--max_fuel 2 --initial_fuel 2 --max_ifuel 2 --initial_ifuel 2 --z3rlimit 30"  
 let lemma_sha256_rnds2 (abef cdgh xmm0:quad32) (t:counter) (block:block_w SHA2_256) : Lemma
   (requires t + 1 < size_k_w SHA2_256 /\
             xmm0.lo0 == v (add_mod (index (k0 SHA2_256) t)     (ws_opaque SHA2_256 block t)) /\
@@ -70,7 +121,31 @@ let lemma_sha256_rnds2 (abef cdgh xmm0:quad32) (t:counter) (block:block_w SHA2_2
   reveal_opaque ws;
   reveal_opaque shuffle_core;
   reveal_opaque make_hash_def;
+  let hash0 = make_hash abef cdgh in
+  let hash1 = shuffle_core_opaque SHA2_256 block hash0 t in
+  let hash1' = shuffle_core SHA2_256 block hash0 t in
+  let hash2 = shuffle_core_opaque SHA2_256 block hash1 t in
   make_hash_properties abef cdgh;
+  let a1,b1,c1,d1,e1,f1,g1,h1 = sha256_rnds2_spec_update 
+                 hash0.[0]
+                 hash0.[1]
+                 hash0.[2]
+                 hash0.[3]
+                 hash0.[4]
+                 hash0.[5]
+                 hash0.[6]
+                 hash0.[7]
+                 (uint_to_t xmm0.lo0) 
+  in
+  //assert_norm (hash0.[0] == b1);  // Fails
+  assert (b1 == hash0.[0]);   // Passes
+  //assert (b1 == hash1'.[1]);  // Fails
+  assert_norm (b1 == hash1'.[1]); 
+//  assert_norm (hash1'.[1] == b1);
+
   make_hash_properties (sha256_rnds2_spec cdgh abef xmm0) abef;
-  //admit();
+  
+  admit();
   ()
+  
+//#pop-options
